cleaning up Rtac notations.
- BREAKING CHANGE, reify_expr_bind and reify_expr now use [[ ]] instead of [[ ]]

examples/Cancel/CancelTac.v
@@ -116,15 +116,12 @@ Section canceller.
 (*  Context {RL10 : ReifiedLemma refl}. *)
 
   Definition EAPPLY : Lemma.lemma typ (expr typ func) (expr typ func) -> rtac typ (expr typ func) :=
-    @EAPPLY _ _ _ _ _ _ (fun subst Ssubst SUsubst => @exprUnify subst _ _ _ _ _ Ssubst SUsubst 30).
+    EAPPLY (fun subst Ssubst SUsubst => @exprUnify subst _ _ _ _ _ Ssubst SUsubst 30).
   Definition APPLY : Lemma.lemma typ (expr typ func) (expr typ func) -> rtac typ (expr typ func) :=
-    @APPLY _ _ _ _ _ _ (fun subst Ssubst SUsubst => @exprUnify subst _ _ _ _ _ Ssubst SUsubst 30).
-  Definition ON_EACH : list (rtac typ (expr typ func)) -> rtacK typ (expr typ func) :=
-    ON_EACH.
-  Definition ON_ALL : rtac typ (expr typ func) -> rtacK typ (expr typ func) := ON_ALL.
+    APPLY (fun subst Ssubst SUsubst => @exprUnify subst _ _ _ _ _ Ssubst SUsubst 30).
 
   Local Instance RtacSound_EAPPLY l (RL : ReifiedLemma l)
-  : RtacSound _ _ (EAPPLY l).
+  : RtacSound (EAPPLY l).
   Proof.
     constructor.
     eapply EAPPLY_sound; eauto with typeclass_instances.
@@ -132,37 +129,29 @@ Section canceller.
   Qed.
 
   Local Instance RtacSound_APPLY l (RL : ReifiedLemma l)
-  : RtacSound _ _ (APPLY l).
+  : RtacSound (APPLY l).
   Proof.
     constructor.
     eapply APPLY_sound; eauto with typeclass_instances.
     intros. eapply exprUnify_sound; eauto with typeclass_instances.
   Qed.
 
-  Lemma ON_EACH_sound
-  : forall ls, Forall rtac_sound ls -> rtacK_sound (ON_EACH ls).
-  Proof. eapply ON_EACH_sound. Qed.
-  Lemma ON_ALL_sound : forall t, rtac_sound t -> rtacK_sound (ON_ALL t).
-  Proof. eapply ON_ALL_sound. Qed.
-
   Variable SOLVER : rtac typ (expr typ func).
-  Variable RtacSound_SOLVER : RtacSound _ _ SOLVER.
+  Variable RtacSound_SOLVER : RtacSound SOLVER.
 
   Notation "'delay' x" := (fun y => x y) (at level 3).
 
   Fixpoint iter_right (Q : expr typ func) : rtac typ (expr typ func) :=
-    FIRST (EAPPLY lem_plus_unit_c ::
-           delay match Q with
-                   | App (App _ L) R => (* guess star *)
-                     FIRST (   THEN (EAPPLY lem_plus_assoc_c1) (delay (ON_ALL (iter_right L)))
-                            :: THEN (EAPPLY lem_plus_assoc_c2) (delay (ON_ALL (iter_right R)))
-                            :: THEN (EAPPLY lem_plus_cancel)
-                                    (ON_EACH (SOLVE SOLVER :: IDTAC :: nil))
-                            :: nil)
+    FIRST [ EAPPLY lem_plus_unit_c
+          | delay match Q with
+                  | App (App _ L) R => (* guess star *)
+                    FIRST [ EAPPLY lem_plus_assoc_c1 ;; delay (ON_ALL (iter_right L))
+                          | EAPPLY lem_plus_assoc_c2 ;; delay (ON_ALL (iter_right R))
+                          | EAPPLY lem_plus_cancel ;; ON_EACH (SOLVE SOLVER :: IDTAC :: nil)
+                          ]
                    | _ =>
-                     THEN (EAPPLY lem_plus_cancel)
-                          (ON_EACH (SOLVE SOLVER :: IDTAC :: nil))
-                 end :: nil).
+                     EAPPLY lem_plus_cancel ;; ON_EACH [ SOLVE SOLVER | IDTAC ]
+                 end ].
 
   Opaque FIRST APPLY EAPPLY.
 
@@ -171,13 +160,11 @@ Section canceller.
 
   Lemma body_non_c
   : rtac_sound
-     (FIRST
-        (EAPPLY lem_plus_unit_c
-         :: delay (THEN (EAPPLY lem_plus_cancel)
-                     (ON_EACH (SOLVE SOLVER :: IDTAC :: nil))) :: nil)).
+     (FIRST [ EAPPLY lem_plus_unit_c
+            | delay (EAPPLY lem_plus_cancel ;;
+                     ON_EACH [ SOLVE SOLVER | IDTAC ]) ]).
   Proof.
     intros. rtac_derive_soundness_default.
-    eapply ON_EACH_sound. rtac_derive_soundness_default.
   Qed.
 
   Lemma iter_right_sound : forall Q, rtac_sound (iter_right Q).
@@ -193,23 +180,22 @@ Section canceller.
     - eapply H.
       eapply TransitiveClosure.LTFin; eauto.
       eapply acc_App_r.
-    - eapply ON_EACH_sound. rtac_derive_soundness_default.
   Qed.
 
   Section afterwards.
     Variable k : rtac typ (expr typ func).
     Fixpoint iter_left (P : expr typ func) : rtac typ (expr typ func) :=
-      FIRST (EAPPLY lem_plus_unit_p ::
-             delay match P with
-                     | App (App _ L) R => (* guess star *)
-                       FIRST (   THEN (EAPPLY lem_plus_assoc_p1) (delay (ON_ALL (iter_left L)))
-                              :: THEN (EAPPLY lem_plus_assoc_p2) (delay (ON_ALL (iter_left R)))
-                              :: k
-                              :: nil)
+      FIRST [ EAPPLY lem_plus_unit_p
+            | delay match P with
+                    | App (App _ L) R => (* guess star *)
+                      FIRST [ EAPPLY lem_plus_assoc_p1 ;; delay (ON_ALL (iter_left L))
+                            | EAPPLY lem_plus_assoc_p2 ;; delay (ON_ALL (iter_left R))
+                            | k
+                            ]
                      | _ => k
-                   end :: nil).
+                   end ].
     Hypothesis k_sound : rtac_sound k.
-    Lemma body_non_p : rtac_sound (FIRST (EAPPLY lem_plus_unit_p :: delay k :: nil)).
+    Lemma body_non_p : rtac_sound (FIRST [ EAPPLY lem_plus_unit_p | delay k ]).
     Proof. rtac_derive_soundness_default. Qed.
 
     Lemma iter_left_sound : forall Q, rtac_sound (iter_left Q).
@@ -231,17 +217,18 @@ Section canceller.
     let k :=
         match Q with
           | App (App _ A) B =>
-            FIRST (   THEN (EAPPLY lem_plus_comm_c) (delay (ON_ALL (iter_right B)))
-                   :: iter_right A
-                   :: nil)
+            FIRST [ EAPPLY lem_plus_comm_c ;; delay (ON_ALL (iter_right B))
+                  | iter_right A
+                  ]
           | _ => FAIL
         end
     in
     match P with
       | App (App _ A) B =>
-        FIRST (   iter_left k A
-               :: THEN FAIL (ON_ALL (THEN (EAPPLY lem_plus_comm_p) (delay (ON_ALL (iter_left k B)))))
-               :: nil)
+        FIRST [ iter_left k A
+              | (* TODO(gmalecha): What is the purpose of this line? *)
+                FAIL ;; ON_ALL (THEN (EAPPLY lem_plus_comm_p) (delay (ON_ALL (iter_left k B))))
+              ]
       | _ => FAIL
     end.
 
@@ -264,16 +251,16 @@ Section canceller.
 
   Definition cancel : rtac typ (expr typ func) :=
     AT_GOAL (fun _ _ e =>
-    REPEAT (size e) (FIRST (   SOLVER
-                      :: THEN (AT_GOAL (fun _ _ e =>
+               REPEAT (size e)
+                      (FIRST [ SOLVER
+                             | AT_GOAL (fun _ _ e =>
                                           match e with
-                                            | App (App _ L) R =>
-                                              FIRST (   THEN (cancel' L R)
-                                                             (ON_ALL (TRY SOLVER))
-                                                     :: nil)
-                                            | _ => FAIL
-                                          end)) (@MINIFY _ _ _ _ _)
-                     :: nil))).
+                                          | App (App _ L) R =>
+                                            FIRST [ cancel' L R ;;
+                                                    ON_ALL (TRY SOLVER) ]
+                                          | _ => FAIL
+                                          end) ;; MINIFY
+                             ])).
 
   Theorem cancel_sound : rtac_sound cancel.
   Proof.
