examples/RTac/EvenOddConst.v
@@ -48,55 +48,46 @@ Definition OE_syn : Lemma.lemma typ (expr typ func) (expr typ func) :=
  |}.
 
 Local Existing Instance Simple.RType_typ.
-Print RSym.
 Definition RSym_nat : @RSym typ _ nat :=
 {| typeof_sym := fun _ => Some tyNat
  ; symD := fun x => x
  ; sym_eqb := fun x y => Some (EqNat.beq_nat x y)
  |}.
 
-
 Local Instance RSym_func : RSym func := RSym_sum (@RSym_func _ _ args) RSym_nat.
 Local Instance RSymOk_func : RSymOk RSym_func := @RSymOk_sum _ _ _ _ _ _ _ _.
-admit.
+constructor. simpl.
+intros. case PeanoNat.Nat.eqb_spec; auto.
 Defined.
 
 Local Instance Expr_expr : Expr _ (expr typ func) := @Expr_expr typ func _ _ _.
 Local Instance ExprOk_expr : @ExprOk _ _ (expr typ func) _ := @ExprOk_expr typ func _ _ _ _ _ _.
-(*
-Definition subst :=
-  FMapSubst.SUBST.raw (expr typ func).
-Local Instance Subst_subst : SubstI.Subst subst (expr typ func)
-  := FMapSubst.SUBST.Subst_subst _.
-Local Instance SubstUpdate_subst : SubstI.SubstUpdate subst (expr typ func)
-  := @FMapSubst.SUBST.SubstUpdate_subst _ _.
-*)
+
+Instance ReifiedLemma_E0_syn : ReifiedLemma E0_syn := { ReifiedLemma_proof := E0 }.
+Instance ReifiedLemma_EO_syn : ReifiedLemma EO_syn := { ReifiedLemma_proof := EO }.
+Instance ReifiedLemma_OE_syn : ReifiedLemma OE_syn := { ReifiedLemma_proof := OE }.
 
 Let APPLY_no_minify (l : Lemma.lemma typ (expr typ func) (expr typ func)) : rtac typ (expr typ func) :=
-  (@APPLY typ (expr typ func) _ _ _ _
-          (fun subst _ _ => @exprUnify subst typ _ Simple.RType_typ _ _ _ _ 10) l).
+  APPLY (fun subst _ _ => @exprUnify subst typ _ Simple.RType_typ _ _ _ _ 10) l.
 
 
 Let APPLY (l : Lemma.lemma typ (expr typ func) (expr typ func)) : rtac typ (expr typ func) :=
-  THEN (APPLY_no_minify l)
-       (@MINIFY _ _ _ _ _).
+  THEN (APPLY_no_minify l) MINIFY.
 
 Theorem APPLY_sound
 : forall l,
-    @Lemma.lemmaD _ _ _ _ _ (exprD'_typ0 (T:=Prop)) _ nil nil l ->
+    ReifiedLemma l ->
     rtac_sound (APPLY l).
 Proof.
-  intros. eapply THEN_sound.
-  eapply APPLY_sound; eauto with typeclass_instances.
-  2: eapply MINIFY_sound.
-  intros. eapply exprUnify_sound; eauto with typeclass_instances.
+  intros. unfold APPLY.
+  eapply THEN_sound; eauto using MINIFY_sound with typeclass_instances.
+  eapply APPLY_sound; eauto using exprUnify_sound, APPLY_sound, MINIFY_sound with typeclass_instances.
 Qed.
 
 Definition even_odd_tac : rtac typ (expr typ func) :=
-  REPEAT 2000 (FIRST (APPLY E0_syn ::
-                      APPLY EO_syn ::
-                      APPLY OE_syn :: nil)).
-
+  REPEAT 2000 (FIRST [ APPLY E0_syn
+                     | APPLY EO_syn
+                     | APPLY OE_syn ]).
 
 Definition build_n (n : nat) : expr typ func := Inj (inr n).
 
@@ -108,14 +99,12 @@ Definition runRTac_empty_goal (tac : rtac typ (expr typ func))
 
 Theorem even_odd_tac_sound
 : rtac_sound even_odd_tac.
+Proof.
   eapply REPEAT_sound.
   eapply FIRST_sound.
-  econstructor; [ eapply APPLY_sound; exact E0 | ].
-  constructor; [ eapply APPLY_sound; exact EO | ].
-  constructor; [ eapply APPLY_sound; exact OE | ].
-  constructor.
+  repeat first [ econstructor; [ eapply APPLY_sound; eauto with typeclass_instances | ]
+               | solve [ constructor ] ].
 Qed.
-
 
 (*Time Eval vm_compute in runRTac_empty_goal even_odd_tac (App Even_syn (build_n 1024)).*)
 
@@ -123,19 +112,39 @@ Definition GoalD (us vs : env) (g : Goal typ (expr typ func)) : Prop :=
   let (tus, us0) := split_env us in
   let (tvs, vs0) := split_env vs in
   match @goalD typ (expr typ func) _ _ _ tus tvs g with
-    | Some P => P us0 vs0
-    | None => False
+  | Some P => P us0 vs0
+  | None => True
   end.
 
 Definition full_solved : @Result typ (expr typ func) (CTop nil nil) :=
   Solved (TopSubst (expr typ func) nil nil).
+
+Theorem generic_soundness
+: forall tac,
+    rtac_sound tac ->
+    forall e,
+    runRTac_empty_goal tac e = full_solved ->
+    GoalD nil nil (GGoal e).
+Proof.
+  intros. unfold rtac_sound, runRTac_empty_goal in *.
+  eapply H in H0.
+  simpl in H0.
+  destruct H0.
+  - constructor.
+  - constructor.
+  - red. simpl.
+    destruct (Ctx.propD nil nil e).
+    + destruct H1; auto.
+    + auto.
+Qed.
 
 Theorem runGoal_sound
 : forall e,
     runRTac_empty_goal even_odd_tac e = full_solved ->
     GoalD nil nil (GGoal e).
 Proof.
-Admitted.
+  intros; eapply generic_soundness; eauto using even_odd_tac_sound.
+Qed.
 
 Let Const (n : nat) : expr typ func := ExprCore.Inj (inr n).
 
@@ -157,44 +166,57 @@ Definition pOE_syn (n : nat) : Lemma.lemma typ (expr typ func) (expr typ func) :
  ; Lemma.concl := App Odd_syn (Const (S n))
  |}.
 
+Instance ReifiedLemma_pE0_syn : ReifiedLemma pE0_syn := { ReifiedLemma_proof := E0 }.
+Instance ReifiedLemma_pEO_syn n : ReifiedLemma (pEO_syn n) := { ReifiedLemma_proof := EO n }.
+Instance ReifiedLemma_pOE_syn n : ReifiedLemma (pOE_syn n) := { ReifiedLemma_proof := OE n }.
+
 Definition even_odd_tac_nrec (fuel : nat) : rtac typ (expr typ func) :=
-  @REC _ _ fuel
-       (fun tac =>
-          AT_GOAL (fun _ _ e =>
-                     match e with
-                       | App (ExprCore.Inj (inl 3%positive))
-                             (ExprCore.Inj (inr 0)) =>
-                         APPLY pE0_syn
-                       | App (ExprCore.Inj (inl 3%positive))
-                             (ExprCore.Inj (inr (S n))) =>
-                         THEN (APPLY (pEO_syn n)) (runOnGoals tac)
-                       | App (ExprCore.Inj (inl 4%positive))
-                             (ExprCore.Inj (inr (S n))) =>
-                         THEN (APPLY (pOE_syn n)) (runOnGoals tac)
-                       | _ => FAIL
-                     end))
+  REC fuel
+      (fun tac =>
+         AT_GOAL (fun _ _ e =>
+                    match e with
+                    | App (ExprCore.Inj (inl 3%positive))
+                          (ExprCore.Inj (inr 0)) =>
+                      APPLY pE0_syn
+                    | App (ExprCore.Inj (inl 3%positive))
+                          (ExprCore.Inj (inr (S n))) =>
+                      APPLY (pEO_syn n) ;; runOnGoals tac
+                    | App (ExprCore.Inj (inl 4%positive))
+                          (ExprCore.Inj (inr (S n))) =>
+                      APPLY (pOE_syn n) ;; runOnGoals tac
+                    | _ => FAIL
+                    end))%rtac
        FAIL.
 
 Fixpoint even_odd_tac_mf (n : nat) : rtac typ (expr typ func) :=
   match n with
-    | 0 => APPLY pE0_syn
-    | S n => THEN (FIRST (APPLY (pEO_syn n) :: APPLY (pOE_syn n) :: nil))
-                  (fun x => runOnGoals (even_odd_tac_mf n) x)
-  end.
+  | 0 => APPLY pE0_syn
+  | S n => FIRST [ APPLY (pEO_syn n) | APPLY (pOE_syn n) ] ;;
+                 (fun x => runOnGoals (even_odd_tac_mf n) x)
+  end%rtac.
 
 Theorem runGoal_sound_mf
 : forall n,
     runRTac_empty_goal (even_odd_tac_mf n) (App Even_syn (Const n)) = full_solved ->
     GoalD nil nil (GGoal (App Even_syn (Const n))).
 Proof.
-Admitted.
+  intros; eapply generic_soundness; eauto.
+  clear. induction n.
+  { simpl. eapply APPLY_sound; eauto with typeclass_instances. }
+  { Opaque FIRST. simpl.
+    rtac_derive_soundness_default; eapply APPLY_sound; eauto with typeclass_instances. }
+Qed.
 
 Theorem runGoal_sound_nonrec
 : forall n,
-    runRTac_empty_goal (even_odd_tac_mf n) (App Even_syn (Const n)) = full_solved ->
+    runRTac_empty_goal (even_odd_tac_nrec n) (App Even_syn (Const n)) = full_solved ->
     GoalD nil nil (GGoal (App Even_syn (Const n))).
 Proof.
-Admitted.
+  intros; eapply generic_soundness; eauto.
+  unfold even_odd_tac_nrec.
+  rtac_derive_soundness_default;
+  eapply APPLY_sound; eauto with typeclass_instances.
+Qed.
 
 (*
 Time Eval vm_compute in let n := 2000 in runRTac_empty_goal (even_odd_tac_mf n) (App Even_syn (Const n)).
