theories/RTac/Apply.v
@@ -48,3 +48,5 @@ Section parameterized.
   Qed.
 
 End parameterized.
+
+Arguments APPLY {typ expr _ _ _ _} unify lem _ _ _ _ _ _ _ : rename.
